chore: wip

src/Init/Data/BitVec/Basic.lean
@@ -881,12 +881,11 @@ def popCountAuxAnd (x : BitVec w) (n : Nat) :=
   The bitwidth of `x` explictly boundspop the number of recursions, thus bounding the depth of the circuit as well
   correctness of def -/
 def popCountAuxRec {w : Nat} (x : BitVec w) (iter : Nat) : BitVec w :=
-    match h : w - iter with
+  match h : w - iter with
   | 0 => BitVec.ofNat w w
-  | n' + 1 => if x = 0#w then BitVec.ofNat w iter else popCountAuxRec (x &&& (x - 1)) (iter + 1)
-termination_by w - iter
+  | diff' + 1 => if x = 0#w then BitVec.ofNat w iter else popCountAuxRec (x &&& (x - 1)) (iter + 1)
+  termination_by w - iter
 
 /-- Count the number of bits with value one in a bitvec -/
 def popCount{w : Nat} (x : BitVec w) : BitVec w := popCountAuxRec x 0
-
 end BitVec
