src/Std/Tactic/BVDecide/Bitblast/BVExpr/Circuit/Lemmas/Expr.lean
@@ -437,12 +437,13 @@ theorem go_denote_eq (aig : AIG BVBit) (expr : BVExpr w) (assign : Assignment)
       intro idx hidx
       rw [goCache_denote_eq]
       exact hinv
-    · rw [← hres]
-      simp only [eval_un, BVUnOp.eval_popCount, BitVec.popCount]
-      rw [denote_blastPopCount]
-      intro idx hidx
-      rw [goCache_denote_eq]
-      exact hinv
+    · sorry
+      -- rw [← hres]
+      -- simp only [eval_un, BVUnOp.eval_clz, BitVec.clz]
+      -- rw [denote_blastClz]
+      -- intro idx hidx
+      -- rw [goCache_denote_eq]
+      -- exact hinv
   · next h =>
     subst h
     rw [← hres]
